Proved theorems

STLC/Basic.lean
@@ -1,1 +1,401 @@
 -- See `study_plan.md` for the plan.
+
+import Mathlib.Data.Finset.Basic
+import Mathlib.Data.Finset.Max
+
+set_option autoImplicit false
+
+inductive Ty where
+  | base
+  | arrow (dom cod : Ty)
+deriving Repr, DecidableEq
+
+-- structure FVar where
+--   id : Nat
+-- deriving Repr, DecidableEq
+
+def FVar := Nat
+
+instance : Repr FVar := inferInstanceAs (Repr Nat)
+
+instance : ToString FVar := inferInstanceAs (ToString Nat)
+
+instance : DecidableEq FVar := inferInstanceAs (DecidableEq Nat)
+
+instance : LinearOrder FVar := inferInstanceAs (LinearOrder Nat)
+
+def Finset.choose_fresh (s : Finset FVar) : FVar :=
+  if h : s.Nonempty then
+    (s.max' h).succ
+  else
+    Nat.zero
+
+theorem Finset.choose_fresh_spec (s : Finset FVar) : s.choose_fresh ∉ s := by
+  unfold Finset.choose_fresh
+  split
+  next h =>
+    intro h'
+    have := Finset.le_max' s _ h'
+    exact Nat.not_succ_le_self _ this
+  next h =>
+    simp at h
+    simp [h]
+
+def Finset.choose_fresh' (s : Finset FVar) : { x : FVar // x ∉ s } :=
+  ⟨s.choose_fresh, s.choose_fresh_spec⟩
+
+inductive Term where
+  | bvar (k : Nat)
+  | fvar (x : FVar)
+  | app (t₁ t₂ : Term)
+  | lam (t : Term)
+deriving Repr, DecidableEq
+
+namespace Term
+
+def fv (t : Term) : Finset FVar :=
+  match t with
+  | bvar _ => ∅
+  | fvar x => {x}
+  | app t₁ t₂ => t₁.fv ∪ t₂.fv
+  | lam t => t.fv
+
+def openAt (t : Term) (k : Nat) (u : Term) : Term :=
+  match t with
+  | bvar i => if k = i then u else t
+  | fvar _ => t
+  | app t₁ t₂ => app (openAt t₁ k u) (openAt t₂ k u)
+  | lam t => lam (openAt t (k + 1) u)
+
+def openT (t s : Term) : Term := t.openAt 0 s
+
+@[simp]
+theorem openAt_bvar {i k u} : (bvar i).openAt k u = if k = i then u else bvar i := by
+  split
+  next h => simp [openAt, h]
+  next h =>
+    simp [openAt]
+    aesop
+
+@[simp]
+theorem openAt_fvar {x k u} : (fvar x).openAt k u = fvar x := by
+  simp [openAt]
+
+@[simp]
+theorem openAt_app {t₁ t₂ k u} : (app t₁ t₂).openAt k u = app (t₁.openAt k u) (t₂.openAt k u) := by
+  simp [openAt]
+
+@[simp]
+theorem openAt_lam {t k u} : (lam t).openAt k u = lam (t.openAt (k + 1) u) := by
+  simp [openAt]
+
+@[simp]
+theorem openT_bvar {i u} : (bvar i).openT u = if 0 = i then u else bvar i := by
+  simp [openT]
+
+@[simp]
+theorem openT_fvar {x u} : (fvar x).openT u = fvar x := by
+  simp [openT]
+
+@[simp]
+theorem openT_app {t₁ t₂ u} : (app t₁ t₂).openT u = app (t₁.openT u) (t₂.openT u) := by
+  simp [openT]
+
+@[simp]
+theorem openT_lam {t u} : (lam t).openT u = lam (t.openAt 1 u) := by
+  simp [openT]
+
+def closeAt (t : Term) (x : FVar) (k : Nat) : Term :=
+  match t with
+  | bvar _ => t
+  | fvar y => if x = y then bvar k else t
+  | app t₁ t₂ => app (closeAt t₁ x k) (closeAt t₂ x k)
+  | lam t => lam (closeAt t x (k + 1))
+
+def close (t : Term) (x : FVar) : Term := closeAt t x 0
+
+@[simp]
+theorem closeAt_bvar {i x k} : (bvar i).closeAt x k = bvar i := by
+  simp [closeAt]
+
+@[simp]
+theorem closeAt_fvar {y x k} : (fvar y).closeAt x k = if x = y then bvar k else fvar y := by
+  simp [closeAt]
+
+@[simp]
+theorem closeAt_app {t₁ t₂ x k} : (app t₁ t₂).closeAt x k = app (t₁.closeAt x k) (t₂.closeAt x k) := by
+  simp [closeAt]
+
+@[simp]
+theorem closeAt_lam {t x k} : (lam t).closeAt x k = lam (t.closeAt x (k + 1)) := by
+  simp [closeAt]
+
+@[simp]
+theorem close_bvar {i x} : (bvar i).close x = bvar i := by
+  simp [close]
+
+@[simp]
+theorem close_fvar {x y} : (fvar x).close y = if y = x then bvar 0 else fvar x := by
+  simp [close]
+
+@[simp]
+theorem close_app {t₁ t₂ x} : (app t₁ t₂).close x = app (t₁.close x) (t₂.close x) := by
+  simp [close]
+
+@[simp]
+theorem close_lam {t x} : (lam t).close x = lam (t.closeAt x 1) := by
+  simp [close]
+
+def subst (t : Term) (x : FVar) (u : Term) : Term :=
+  match t with
+  | bvar _ => t
+  | fvar y => if x = y then u else t
+  | app t₁ t₂ => app (subst t₁ x u) (subst t₂ x u)
+  | lam t => lam (subst t x u)
+
+@[simp]
+theorem subst_bvar {k x u} : (bvar k).subst x u = bvar k := by
+  simp [subst]
+
+@[simp]
+theorem subst_fvar {y x u} : (fvar y).subst x u = if x = y then u else fvar y := by
+  simp [subst]
+
+@[simp]
+theorem subst_app {t₁ t₂ x u} : (app t₁ t₂).subst x u = app (t₁.subst x u) (t₂.subst x u) := by
+  simp [subst]
+
+@[simp]
+theorem subst_lam {t x u} : (lam t).subst x u = lam (t.subst x u) := by
+  simp [subst]
+
+inductive LC : Term → Prop where
+  | lc_fvar (x : FVar) : LC (.fvar x)
+  | lc_app {t₁ t₂ : Term} (h₁ : LC t₁) (h₂ : LC t₂) : LC (.app t₁ t₂)
+  | lc_lam {t : Term} (L : Finset FVar) (h : ∀ x ∉ L, LC (t.openT (.fvar x))) : LC (.lam t)
+
+def IsBody (t : Term) : Prop := ∃ L : Finset FVar, ∀ x ∉ L, (t.openT (.fvar x)).LC
+
+@[simp]
+theorem LC.fvar {x : FVar} : LC (.fvar x) := by
+  exact .lc_fvar x
+
+@[simp]
+theorem LC.app_iff {t₁ t₂ : Term} : LC (.app t₁ t₂) ↔ LC t₁ ∧ LC t₂ := by
+  apply Iff.intro
+  . intro h
+    match h with
+    | .lc_app h₁ h₂ => exact ⟨h₁, h₂⟩
+  . intro ⟨h₁, h₂⟩
+    exact .lc_app h₁ h₂
+
+@[simp]
+theorem LC.lam_iff {t : Term} : t.lam.LC ↔ t.IsBody := by
+  apply Iff.intro
+  . intro lc
+    match lc with
+    | .lc_lam L h => exact ⟨L, h⟩
+  . intro ⟨L, h⟩
+    exact .lc_lam L h
+
+theorem openAt_eq_of_LCAux {t u v : Term} {i j : Nat} (ne : i ≠ j) (h : (t.openAt i u).openAt j v = t.openAt i u) :
+  t.openAt j v = t := by
+  induction t generalizing i j with
+  | bvar k =>
+    simp
+    intro eq
+    subst k
+    simp [ne] at h
+    simp [h]
+  | fvar x => simp
+  | app t₁ t₂ ih₁ ih₂ =>
+    simp at h
+    simp [ih₁, ih₂]
+    exact ⟨ih₁ ne h.1, ih₂ ne h.2⟩
+  | lam t ih =>
+    simp at h
+    simp
+    exact ih (by omega) h
+
+theorem openAt_eq_of_LC {t : Term} {k : Nat} {u : Term} (lc : t.LC) :
+  t.openAt k u = t := by
+  induction lc generalizing k with
+  | lc_fvar x => simp
+  | lc_app h₁ h₂ ih₁ ih₂ => simp [ih₁, ih₂]
+  | @lc_lam t L h ih =>
+    let x := L.choose_fresh
+    simp
+    apply openAt_eq_of_LCAux (by omega) (ih x L.choose_fresh_spec)
+
+theorem openAt_subst {t u w : Term} {x : FVar} {i : Nat} (lc : u.LC) :
+  (t.openAt i w).subst x u = (t.subst x u).openAt i (w.subst x u) := by
+  induction t generalizing i with
+  | bvar k =>
+    if h : i = k then
+      simp [h]
+    else
+      simp [h]
+  | fvar z =>
+    if h : x = z then
+      simp [h, openAt_eq_of_LC lc]
+    else
+      simp [h]
+  | app t₁ t₂ ih₁ ih₂ =>
+    simp [ih₁, ih₂]
+  | lam t ih =>
+    simp [ih]
+
+theorem open_subst {t u w : Term} {x : FVar} (lc : u.LC) :
+  (t.openT w).subst x u = (t.subst x u).openT (w.subst x u) :=
+  openAt_subst lc
+
+theorem openAt_var_subst {t u : Term} {x y : FVar} {i : Nat} (ne : x ≠ y) (lc : u.LC) :
+  (t.openAt i (fvar y)).subst x u = (t.subst x u).openAt i (fvar y) := by
+  calc (t.openAt i (fvar y)).subst x u
+    _ = (t.subst x u).openAt i ((fvar y).subst x u) := openAt_subst lc
+    _ = (t.subst x u).openAt i (fvar y) := by simp [ne]
+
+theorem open_var_subst {t u : Term} {x y : FVar} (ne : x ≠ y) (lc : u.LC) :
+  (t.openT (fvar y)).subst x u = (t.subst x u).openT (fvar y) :=
+  openAt_var_subst ne lc
+
+theorem subst_fresh {t : Term} {x : FVar} {u : Term} (h : x ∉ t.fv) : t.subst x u = t := by
+  induction t with
+  | bvar k => rfl
+  | fvar y =>
+    simp [fv] at h
+    simp [subst, h]
+  | app t₁ t₂ ih₁ ih₂ =>
+    simp [fv] at h
+    simp [h] at ih₁ ih₂
+    simp [subst, ih₁, ih₂]
+  | lam t ih =>
+    simp [fv] at h
+    simp [subst, ih h]
+
+theorem subst_intro' {t : Term} {k : Nat} {x : FVar} {u : Term} (h : x ∉ t.fv) :
+  (t.openAt k (.fvar x)).subst x u = t.openAt k u := by
+  induction t generalizing k with
+  | bvar i =>
+    if h' : k = i then
+      simp [h']
+    else
+      simp [h']
+  | fvar y =>
+    simp [fv] at h
+    simp [h]
+  | app t₁ t₂ ih₁ ih₂ =>
+    simp [fv] at h
+    simp [h] at ih₁ ih₂
+    simp [ih₁, ih₂]
+  | lam t ih =>
+    simp [fv] at h
+    simp [h] at ih
+    simp [ih]
+
+theorem subst_intro {t : Term} {x : FVar} {u : Term} (h : x ∉ t.fv) :
+  (t.openT (.fvar x)).subst x u = t.openT u :=
+  subst_intro' h
+
+theorem LC_subst {t u : Term} {x : FVar} (lc₁ : t.LC) (lc₂ : u.LC) : (t.subst x u).LC := by
+  induction lc₁ with
+  | lc_fvar y =>
+    simp
+    split <;> simp [lc₂]
+  | lc_app h₁ h₂ ih₁ ih₂ => simp [ih₁, ih₂]
+  | @lc_lam t L h ih =>
+    simp
+    exists L ∪ {x}
+    intro y hy
+    simp at hy
+    have ne : x ≠ y := fun eq => by simp [eq] at hy
+    rw [←open_var_subst ne lc₂]
+    apply ih y hy.1
+
+theorem LC_open_body {t u : Term} (h : t.IsBody) (lc : u.LC) : (t.openT u).LC := by
+  have ⟨L, hL⟩ := h
+  let L' := L ∪ t.fv
+  let ⟨x, hx⟩ := L'.choose_fresh'
+  simp [L'] at hx
+  rw [←subst_intro hx.2]
+  apply LC_subst ?_ lc
+  exact hL x hx.1
+
+inductive IsValue : Term → Prop where
+  | value_lam {t : Term} (h : t.IsBody) : IsValue (.lam t)
+
+inductive Cbv : Term → Term → Prop where
+  | cbv_beta {t u : Term} (h : t.IsBody) (val : u.IsValue) : Cbv (.app (.lam t) u) (t.openT u)
+  | cbv_app_left {t t' u : Term} (h : Cbv t t') (lc : u.LC) : Cbv (.app t u) (.app t' u)
+  | cbv_app_right {t u u' : Term} (val : t.IsValue) (h : Cbv u u') : Cbv (.app t u) (.app t u')
+
+theorem LC_of_value {t : Term} (val : t.IsValue) : t.LC := by
+  cases val with
+  | value_lam h => simp [h]
+
+theorem LC_of_cbv {t t' : Term} (step : Cbv t t') : t.LC ∧ t'.LC := by
+  induction step with
+  | cbv_beta h val => simp [h, val, LC_of_value, LC_open_body]
+  | cbv_app_left h lc ih => simp [ih, lc]
+  | cbv_app_right val h ih => simp [ih, LC_of_value val]
+
+theorem no_cbv_of_value {t t' : Term} (val : t.IsValue) : ¬ Cbv t t' := by
+  intro step
+  nomatch val, step
+
+theorem cbv_deterministic {t t' t'' : Term} (step₁ : Cbv t t') (step₂ : Cbv t t'') : t' = t'' := by
+  induction step₁ generalizing t'' with
+  | cbv_beta h₁ val₁ =>
+    cases step₂ with
+    | cbv_beta h₂ val₂ => rfl
+    | cbv_app_left h₂ lc₂ => exact False.elim (no_cbv_of_value (.value_lam h₁) h₂)
+    | cbv_app_right val₂ h₂ => exact False.elim (no_cbv_of_value val₁ h₂)
+  | cbv_app_left h₁ lc₁ ih₁ =>
+    cases step₂ with
+    | cbv_beta h₂ val₂ => exact False.elim (no_cbv_of_value (.value_lam h₂) h₁)
+    | cbv_app_left h₂ lc₂ => simp [ih₁ h₂]
+    | cbv_app_right val₂ h₂ => exact False.elim (no_cbv_of_value val₂ h₁)
+  | cbv_app_right val₁ h₁ ih₁ =>
+    cases step₂ with
+    | cbv_beta h₂ val₂ => exact False.elim (no_cbv_of_value val₂ h₁)
+    | cbv_app_left h₂ lc₂ => exact False.elim (no_cbv_of_value val₁ h₂)
+    | cbv_app_right val₂ h₂ => simp [ih₁ h₂]
+
+end Term
+
+def TyCtx := List (FVar × Ty)
+
+instance : Repr TyCtx := inferInstanceAs (Repr (List (FVar × Ty)))
+
+instance : DecidableEq TyCtx := inferInstanceAs (DecidableEq (List (FVar × Ty)))
+
+instance : Membership (FVar × Ty) TyCtx := inferInstanceAs (Membership (FVar × Ty) (List (FVar × Ty)))
+
+namespace TyCtx
+
+def dom (Γ : TyCtx) : List FVar := Γ.map (·.1)
+
+inductive ok : TyCtx → Prop where
+  | ok_nil : ok []
+  | ok_cons {x : FVar} {T : Ty} {Γ : TyCtx} (h₁ : x ∉ Γ.dom) (h₂ : ok Γ) : ok ((x, T) :: Γ)
+
+end TyCtx
+
+namespace Term
+
+inductive HasType : TyCtx → Term → Ty → Prop where
+  | type_var {Γ : TyCtx} {x : FVar} {T : Ty} (ok : Γ.ok) (mem : (x, T) ∈ Γ) : HasType Γ (.fvar x) T
+  | type_app {Γ : TyCtx} {t₁ t₂ : Term} {T₁ T₂ : Ty}
+    (h₁ : HasType Γ t₁ (T₁.arrow T₂)) (h₂ : HasType Γ t₂ T₁) : HasType Γ (.app t₁ t₂) T₂
+  | type_lam {Γ : TyCtx} {t : Term} {T₁ T₂ : Ty} (L : Finset FVar)
+    (h : ∀ x ∉ L, HasType (Γ.cons (x, T₁)) (t.openT (.fvar x)) T₂) : HasType Γ (.lam t) (T₁.arrow T₂)
+
+theorem LC_of_hasType {Γ : TyCtx} {t : Term} {T : Ty} (typing : t.HasType Γ T) : t.LC := by
+  induction typing with
+  | type_var ok mem => simp
+  | type_app h₁ h₂ ih₁ ih₂ => simp [ih₁, ih₂]
+  | type_lam L h ih =>
+    simp
+    exact ⟨L, ih⟩
+
+end Term
